seq_adequacy theorem

src/sequential/SeqLiftStep.v
@@ -35,8 +35,10 @@ Require Import Delayed.
 
 Require Import Lia.
 
+Require Import JoinedView.
 Require Import SeqLift.
-(* Require Import Simple. *)
+Require Import gSimulation.
+Require Import Simple.
 
 
 Record sim_tview
@@ -781,3 +783,114 @@ Proof.
   }
   { i. eapply SIM. }
 Qed.
+
+Variant initial_finalized: Messages.t :=
+| initial_finalized_intro
+    loc
+  :
+    initial_finalized loc Time.bot Time.bot Message.elt
+.
+
+Lemma configuration_initial_finalized s
+  :
+    finalized (Configuration.init s) = initial_finalized.
+Proof.
+  extensionality loc.
+  extensionality from.
+  extensionality to.
+  extensionality msg.
+  apply Coq.Logic.PropExtensionality.propositional_extensionality.
+  split; i.
+  { inv H. ss. unfold Memory.init, Memory.get in GET.
+    rewrite Cell.init_get in GET. des_ifs. }
+  { inv H. econs; eauto. i. ss. unfold Threads.init in *.
+    rewrite IdentMap.Facts.map_o in TID. unfold option_map in *. des_ifs.
+  }
+Qed.
+
+Definition initial_mapping: Mapping.t :=
+  Mapping.mk
+    (fun v ts =>
+       if PeanoNat.Nat.eq_dec v 0 then
+         if (Time.eq_dec ts Time.bot) then Some (Time.bot)
+         else None
+       else None)
+    0
+    (fun _ ts => ts = Time.bot)
+.
+
+Definition initial_vers: versions :=
+  fun loc ts =>
+    if (Time.eq_dec ts Time.bot) then Some (fun _ => 0) else None.
+
+Section LIFT.
+  Let world := (Mapping.ts * versions)%type.
+
+  Let world_bot: world := (fun _ => initial_mapping, initial_vers).
+
+  Let world_messages_le (msgs: Messages.t) (w0: world) (w1: world): Prop :=
+    let (f0, vers0) := w0 in
+    let (f1, vers1) := w1 in
+    Mapping.les f0 f1 /\ versions_le vers0 vers1.
+
+  Let sim_memory (b: bool) (w: world) (views: Loc.t -> Time.t -> list View.t)
+      (mem_src: Memory.t) (mem_tgt: Memory.t): Prop :=
+    let (f, vers) := w in
+    sim_memory (fun _ => None) f vers mem_src mem_tgt.
+
+  Let sim_timemap (w: world)
+      (tm_src: TimeMap.t) (tm_tgt: TimeMap.t): Prop :=
+    let (f, vers) := w in
+    sim_timemap (fun _ => True) f (Mapping.vers f) tm_src tm_tgt.
+
+  Let sim_local (w: world) (views: Loc.t -> Time.t -> list View.t) (lc_src: Local.t) (lc_tgt: Local.t): Prop :=
+    let (f, vers) := w in
+    sim_local f vers (fun _ => None) (fun _ => None) lc_src lc_tgt.
+
+
+
+  Lemma world_messages_le_PreOrder: forall msgs, PreOrder (world_messages_le msgs).
+  Proof.
+    ii. econs.
+    { ii. red. des_ifs. splits; auto.
+      { refl. }
+      { refl. }
+    }
+    { ii. unfold world_messages_le in *. des_ifs. des. splits; auto.
+      { etrans; eauto. }
+      { etrans; eauto. }
+    }
+  Qed.
+
+  Lemma sim_local_memory_bot:
+    forall w views lc_src lc_tgt
+           (SIM: sim_local w views lc_src lc_tgt)
+           (BOT: (Local.promises lc_tgt) = Memory.bot),
+      (Local.promises lc_src) = Memory.bot.
+  Proof.
+    ii. unfold sim_local in *. des_ifs. inv SIM. ss. subst.
+    inv PROMISES. eapply Memory.ext. ii.
+    rewrite Memory.bot_get.
+    destruct (Memory.get loc ts prom_src) eqn:EQ; auto. destruct p.
+    hexploit SOUND; eauto. i. des; ss. rewrite Memory.bot_get in GET. ss.
+  Qed.
+
+  Lemma world_messages_le_mon:
+    forall msgs0 msgs1 w0 w1
+           (LE: world_messages_le msgs1 w0 w1)
+           (MSGS: msgs0 <4= msgs1),
+      world_messages_le msgs0 w0 w1.
+  Proof.
+    unfold world_messages_le. ii. des_ifs.
+  Qed.
+
+  Lemma sim_lift_gsim lang_src lang_tgt sim_terminal
+        (st_src: lang_src.(Language.state)) (st_tgt: lang_tgt.(Language.state))
+        (SIM: @sim_seq_all _ _ sim_terminal st_src st_tgt)
+    :
+      @sim_thread_past
+        world world_messages_le sim_memory sim_timemap sim_local
+        lang_src lang_tgt sim_terminal false world_bot st_src Local.init TimeMap.bot Memory.init st_tgt Local.init TimeMap.bot Memory.init (JConfiguration.init_views, initial_finalized).
+  Proof.
+  Admitted.
+End LIFT.
